theories/Core/Soundness/ContextCases.v
@@ -12,35 +12,6 @@ Qed.
 #[export]
   Hint Resolve glu_rel_ctx_empty : mcpts.
 
-(* Lemma glu_rel_typ_implies_glu_rel_exp_typ {P} (pred_P : PredicativeSig P) : forall {anns s Γ A}, *)
-(*     {{ ⟪ pred_P ⟫ Γ with anns ⊩ A @ s }} -> *)
-(*     exists so, {{ ⟪ pred_P ⟫ Γ with anns ⊩ A : Sort@s @ so }}. *)
-(* Proof. *)
-(*   intros * [Sb]. *)
-(*   destruct_conjs. *)
-(*   assert (exists env_rel, {{ EF Γ ≈ Γ ∈ per_ctx_env pred_P ↘ env_rel }}) as [env_rel] by mauto 3. *)
-(*   assert (exists ρ ρ', initial_env Γ ρ /\ initial_env Γ ρ' /\ {{ Dom ρ ≈ ρ' ∈ env_rel }}) as [ρ] by mauto using per_ctx_then_per_env_initial_env. *)
-(*   destruct_conjs. *)
-(*   functional_initial_env_rewrite_clear. *)
-(*   assert {{ Γ ⊢s Id ® ρ ∈ Sb }} by (eapply initial_env_glu_rel_exp; mauto 3). *)
-(*   assert (glu_rel_typ_with_sub pred_P s Γ A {{{ Id }}} ρ) by mauto 3. *)
-(*   dependent destruction H4. *)
-(*   eexists. *)
-(*   econstructor; split; mauto 3. *)
-(*   intros. *)
-(*   invert_glu_ *)
-  
-(*   destruct H. *)
-(*   eexists; econstructor; mauto 3. *)
-(*   assert {{ Γ ⊢ A[σ] : Sort@s }} by (eapply glu_sort_elem_sort_lvl; mauto 3). *)
-(*   gen_presup H3. *)
-(*   assert (exists Δ K s', {{ Γ ⊢s σ : Δ }} /\ {{ Δ ⊢ A : K }} /\ *)
-(*                       (({{ Γ ⊢ K[σ] ≈ Sort@s }} /\ {{ Δ ⊢ K : Sort@s' }}) \/ ({{ Γ ⊢ K ≈ Sort@s }} /\ {{ Δ ⊢ K ≈ Sort@s' }}))) as [Δ [K [s'']]] by mauto 2. *)
-(*   destruct_conjs. *)
-(*   repeat split; mauto 3. *)
-(*   repeat eexists; mauto 3. *)
-(* Qed. *)
-
 Lemma glu_rel_typ_to_wf_exp {P} (pred_P : PredicativeSig P) : forall {anns Γ A s},
     {{ ⟪ pred_P ⟫ Γ with anns ⊩ A @ s }} ->
     {{ Γ ⊢ A : Sort@s }}.
