theories/Core/Soundness/FunctionCases.v
@@ -29,96 +29,6 @@ Qed.
 
 Hint Resolve cons_glu_sub_pred_pi_helper : mcpts.
 
-(* Lemma glu_rel_exp_pi {P} (pred_P : PredicativeSig P) (full_P : FullSig P) : forall {Γ A B s1 s2 s3 s1' s2' s3'} {r : Ru P s1 s2 s3}, *)
-(*     Ax P s3 s3' -> *)
-(*     {{ ⟪ pred_P ⟫ Γ ⊩ A : Sort@s1 @ s1'}} -> *)
-(*     {{ ⟪ pred_P ⟫ Γ, A@s1 ⊩ B : Sort@s2 @ s2' }} -> *)
-(*     {{ ⟪ pred_P ⟫ Γ ⊩ Π r A B : Sort@s3 @ s3' }}. *)
-(* Proof. *)
-(*   intros * Hax HA HB. *)
-(*   assert {{ ⟪ pred_P ⟫ ⊩ Γ }} as [SbΓ] by mauto. *)
-(*   assert {{ Γ ⊢ A : Sort@s1 }} by mauto. *)
-(*   inversion_clear HA as [SbΓ' []]. *)
-(*   handle_functional_glu_ctx_env P. *)
-(*   rename SbΓ' into SbΓ. *)
-(*   assert {{ EG Γ, A@s1 ∈ glu_ctx_env pred_P ↘ cons_glu_sub_pred pred_P s1 Γ A SbΓ }} by (econstructor; mauto; reflexivity). *)
-(*   assert {{ Γ, A@s1 ⊢ B : Sort@s2 }} by mauto. *)
-(*   inversion_clear HB as [SbΓA []]. *)
-(*   eapply glu_rel_exp_of_typ; mauto 3. *)
-(*   intros. *)
-(*   assert {{ Δ ⊢s σ : Γ }} by mauto 4. *)
-(*   split; mauto 3. *)
-(*   destruct_glu_rel_exp_with_sub. *)
-(*   simplify_evals. *)
-(*   match_by_head (@glu_sort_elem P) ltac:(fun H => directed invert_glu_sort_elem H). *)
-(*   assert (typ_rel Δ {{{ Sort@s1[σ] }}}) by (eapply glu_sort_elem_trm_typ; mauto 3). *)
-(*   handle_functional_glu_sort_elem P. *)
-(*   unfold sort_glu_typ_pred in *. *)
-(*   unfold sort_glu_exp_pred' in *. *)
-(*   unfold glu_sort_typ_rec in *. *)
-(*   destruct_conjs. *)
-(*   rename m into a. *)
-(*   assert {{ ⟪ pred_P ⟫ Γ ⊨u Π r A B : Sort@s3 }} as [env_relΓ]%rel_exp_unsorted_of_typ_inversion1 by mauto 3 using completeness_fundamental_exp. *)
-(*   assert {{ ⟪ pred_P ⟫ Γ, A@s1 ⊨u B : Sort@s2 }} as [env_relΓA]%rel_exp_unsorted_of_typ_inversion1 by mauto 3 using completeness_fundamental_exp. *)
-(*   destruct_conjs. *)
-(*   match_by_head1 (per_ctx_env pred_P env_relΓA) invert_per_ctx_env. *)
-(*   pose env_relΓA. *)
-(*   assert {{ Dom ρ ≈ ρ ∈ env_relΓ }} by (eapply glu_ctx_env_per_env; revgoals; eassumption). *)
-(*   (on_all_hyp: destruct_rel_by_assumption env_relΓ). *)
-(*   simplify_evals. *)
-(*   eexists; repeat split; mauto. *)
-(*   intros. *)
-(*   match_by_head1 (@glu_sort_elem P) ltac:(fun H => directed invert_glu_sort_elem H). *)
-(*   rename x into OP, x0 into OEL. *)
-(*   rename H11 into IP, H13 into IEL. *)
-(*   assert (per_sort_elem pred_P s1 (head_rel ρ ρ H21) a a) by mauto 2. *)
-(*   handle_per_sort_elem_irrel. *)
-(*   handle_functional_glu_sort_elem P. *)
-(*   econstructor; mauto 3. *)
-(*   - intros. *)
-(*     eapply glu_sort_elem_typ_monotone; mauto 3. *)
-
-(*   - intros Δ' τ **. *)
-(*     assert {{ Δ' ⊢s τ : Δ }} by mauto 2. *)
-(*     assert {{ Dom ρ ↦ m ≈ ρ ↦ m ∈ env_relΓA }} as HrelΓA by (apply_relation_equivalence; mautosolve 2). *)
-(*     apply_relation_equivalence. *)
-(*     (on_all_hyp: fun H => destruct (H _ _ HrelΓA)). *)
-(*     destruct_by_head (@per_sort P). *)
-(*     functional_eval_rewrite_clear. *)
-(*     match goal with *)
-(*     | _: {{ ⟦ B ⟧ ρ ↦ m ↘ ^?a }} |- _ => *)
-(*         rename a into b *)
-(*     end. *)
-(*     assert {{ Δ' ⊢ M : A[σ][τ] }} by mauto 3 using glu_sort_elem_trm_escape. *)
-(*     assert {{ DG b ∈ glu_sort_elem pred_P s2 ↘ OP m equiv_m ↘ OEL m equiv_m }} by mauto 2. *)
-(*     assert {{ Δ' ⊢ B[σ∘τ,,M] ≈ B[q σ][τ,,M] : Sort@s2 }} as <-. *)
-(*     { *)
-(*       gen_presups. *)
-(*       assert {{ Δ' ⊢s q σ ∘ (τ ,, M) ≈ σ ∘ τ ,, M : Γ, A@s1 }} by (eapply sub_decompose_q; mauto 2). *)
-(*       transitivity {{{ B[(q σ)∘(τ,,M)] }}}. *)
-(*       - eapply wf_exp_eq_sub_cong_sort; mauto 3. *)
-(*       - eapply exp_eq_sub_compose_typ_sort; mauto 3. *)
-(*         + eapply sub_q; mauto 2. *)
-(*         + econstructor; mauto 2. *)
-(*     } *)
-(*     assert {{ Δ' ⊢s (σ∘τ),,M ® ρ ↦ m ∈ cons_glu_sub_pred pred_P s1 Γ A SbΓ }} as Hconspred by mauto 2. *)
-(*     handle_functional_glu_ctx_env P. *)
-(*     assert (SbΓA Δ' {{{ σ∘τ,,M }}} d{{{ ρ ↦ m }}}) as Hconspred' by (eapply H30; eassumption). *)
-(*     (on_all_hyp: fun H => destruct (H _ _ _ Hconspred')). *)
-(*     simplify_evals. *)
-(*     match_by_head (@glu_sort_elem P) ltac:(fun H => directed invert_glu_sort_elem H). *)
-(*     apply_predicate_equivalence. *)
-(*     unfold sort_glu_exp_pred' in *. *)
-(*     unfold glu_sort_typ_rec in *. *)
-(*     destruct_conjs. *)
-(*     handle_functional_glu_sort_elem P. *)
-(*     eassumption. *)
-(* Qed. *)
-
-(* #[export] *)
-(* Hint Resolve glu_rel_exp_pi : mcpts. *)
-
-
 Lemma glu_rel_exp_pi_unsorted' {P} (pred_P : PredicativeSig P) : forall {anns Γ A B s1 s2 s3} {r : Ru_pi P s1 s2 s3},
     {{ ⟪ pred_P ⟫ Γ with anns ⊩u A : Sort@s1 @ ^so_None }} ->
     {{ ⟪ pred_P ⟫ Γ, A with (so_Some s1)::anns ⊩u B : Sort@s2 @ ^so_None }} ->
@@ -142,14 +52,7 @@ Proof.
   inversion H11; subst.
   rename s into s1.
   match_by_head (@glu_typ_elem P) ltac:(fun H => directed inversion H); subst.
-  (* match_by_head (@glu_sort_elem P) ltac:(fun H => directed invert_glu_sort_elem H). *)
   simpl_glu_rel.
-  (* assert (typ_rel Δ {{{ Sort@s1[σ] }}}) by (eapply glu_sort_elem_trm_typ; mauto 3).   *)
-  (* handle_functional_glu_sort_elem P. *)
-  (* unfold sort_glu_typ_pred in *. *)
-  (* unfold sort_glu_exp_pred' in *. *)
-  (* unfold glu_sort_typ_rec in *. *)
-  (* destruct_conjs. *)
   rename m into a.
   assert {{ ⟪ pred_P ⟫ Γ ⊨u Π r A B : Sort@s3 }} as [env_relΓ]%rel_exp_unsorted_of_typ_inversion1 by mauto 3 using completeness_fundamental_exp.
   assert {{ ⟪ pred_P ⟫ Γ, A ⊨u B : Sort@s2 }} as [env_relΓA]%rel_exp_unsorted_of_typ_inversion1 by mauto 3 using completeness_fundamental_exp.
@@ -162,8 +65,6 @@ Proof.
   eexists; repeat split; mauto.
   intros.
   unshelve (match_by_head1 (@glu_sort_elem P) ltac:(fun H => directed invert_glu_sort_elem H)); mauto 2.
-  (* rename typ_rel1 into IP', exp_rel1 into IEL'. *)
-  (* rename x into OP', x0 into OEL'. *)
   rename H20 into equiv_ρ_ρ.
   assert (per_sort_elem pred_P s1 (head_rel ρ ρ equiv_ρ_ρ) a a) by mauto 2.
   destruct glu_a.
@@ -208,14 +109,9 @@ Proof.
     pose proof (H5 _ _ _ Hconspred').
     inversion H; subst.
     inversion H33; subst.
-    (* dependent destruction (H5 _ _ _ Hconspred'). *)
-    (* (on_all_hyp: fun H => inversion (H _ _ _ Hconspred')). *)
     simplify_evals.
     match_by_head (@glu_sort_elem P) ltac:(fun H => directed invert_glu_sort_elem H).
     apply_predicate_equivalence.
-    (* unfold sort_glu_exp_pred' in *. *)
-    (* unfold glu_sort_typ_rec in *. *)
-    (* destruct_conjs. *)
     handle_functional_glu_sort_elem P.
     inversion H37; subst.
     simpl_glu_rel.
@@ -339,7 +235,6 @@ Proof.
   do 2 eexists; repeat split; mauto.
   intros.
   unshelve(match_by_head (@glu_sort_elem P) ltac:(fun H => directed invert_glu_sort_elem H)); mauto 2.
-  (* rename H19 into IP, H20 into IEL, x into OP, x0 into OEL. *)
   assert (per_typ_elem pred_P (head_rel ρ ρ H11) a a) by mauto 2.
   
   handle_per_typ_elem_irrel.
@@ -448,22 +343,6 @@ Proof.
     mauto 3.
 Qed.
 
-(* Lemma glu_rel_exp_fn {P} (pred_P : PredicativeSig P) (full_P : FullSig P) : forall {Γ M A B s1 s2 s3 s1'} {r : Ru P s1 s2 s3}, *)
-(*     {{ ⟪ pred_P ⟫ Γ ⊩ A : Sort@s1 @ s1' }} -> *)
-(*     {{ ⟪ pred_P ⟫ Γ, A@s1 ⊩ M : B @ s2 }} -> *)
-(*     {{ ⟪ pred_P ⟫ Γ ⊩ λ r A M : Π r A B @ s3 }}. *)
-(* Proof. *)
-(*   intros * HA HM. *)
-(*   assert (exists s2', {{ ⟪ pred_P ⟫ Γ, A@s1 ⊩ B : Sort@s2 @ s2' }}) as [s2'] by mauto 3. *)
-(*   assert {{ ⟪ pred_P ⟫ ⊩ Γ }} by mauto 3. *)
-(*   assert {{ ⟪ pred_P ⟫ ⊩ Γ, A@s1 }} by mauto 3. *)
-(*   mauto 3 using glu_rel_exp_fn_helper. *)
-(* Qed. *)
-
-(* #[export] *)
-(* Hint Resolve glu_rel_exp_fn : mcpts. *)
-
-
 Lemma glu_rel_exp_fn_helper_unsorted {P} (pred_P : PredicativeSig P) : forall {anns Γ M A B s1 s2 s3} {r : Ru_pi P s1 s2 s3},
     {{ ⟪ pred_P ⟫ Γ with anns ⊩u A : Sort@s1 @ ^so_None }} ->
     {{ ⟪ pred_P ⟫ Γ, A with (so_Some s1)::anns ⊩u B : Sort@s2 @ ^so_None }} ->
@@ -496,21 +375,13 @@ Proof.
   assert {{ Dom ρ ≈ ρ ∈ env_relΓ }} by (eapply glu_ctx_env_per_env; revgoals; eassumption).
   destruct_rel_typ_unsorted.
   destruct_rel_typ.
-  (* assert (glu_rel_exp_with_sub_unsorted pred_P so1 Δ A {{{ Sort@s1 }}} σ ρ) by mauto 2. *)
-  (* dependent destruction H18. *)
-  (* dependent destruction H21. *)
   destruct_glu_rel_exp_with_sub_unsorted.
   simplify_evals.
-  (* match_by_head (@glu_sort_elem P) ltac:(fun H => directed invert_glu_sort_elem H). *)
   match_by_head (@glu_typ_elem P) ltac:(fun H => directed inversion H).
   inversion H21; subst.
   rename s into s1.
   apply_predicate_equivalence.
   simpl_glu_rel.
-  (* unfold sort_glu_exp_pred' in *. *)
-  (* unfold glu_sort_typ_rec in *. *)
-  (* destruct_conjs. *)
-  (* handle_functional_glu_sort_elem P. *)
   do 2 eexists; repeat split; mauto.
   intros.
   unshelve(match_by_head (@glu_sort_elem P) ltac:(fun H => directed invert_glu_sort_elem H)); mauto 2.
@@ -612,7 +483,6 @@ Proof.
     }
     pose proof (H5 _ _ _ HSbΓA).
     dependent destruction H41.
-    (* (on_all_hyp: fun H => destruct (H _ _ _ HSbΓA)). *)
     simplify_evals.
     match_by_head (@glu_sort_elem P) ltac:(fun H => directed invert_glu_sort_elem H).
     handle_functional_glu_sort_elem P.
@@ -679,8 +549,6 @@ Proof.
   handle_functional_glu_ctx_env P.
   eexists; split; [eassumption |].
   intros.
-  (* assert (SbΓ Δ σ ρ) by (eapply H7; mauto 2). *)
-  (* assert (SbΓ' Δ σ ρ) by (eapply H13; mauto 2). *)
   assert (SbΓ Δ σ ρ) by (eapply H6; mauto 2).
   assert (SbΓ' Δ σ ρ) by (eapply H12; mauto 2).
   destruct_glu_rel_exp_with_sub.
@@ -712,7 +580,6 @@ Proof.
   destruct_conjs.
   handle_functional_glu_sort_elem P.
   match_by_head (@per_sort_elem P) ltac:(fun H => directed invert_per_sort_elem H).
-  (* inversion_clear H22. *)
   inversion_clear H21.
   match goal with
   | _: glu_sort_elem pred_P s1 ?P' ?El' a,
@@ -765,7 +632,6 @@ Proof.
   {
     autorewrite with mcpts; eapply glu_sort_elem_typ_unique_upto_exp_eq; revgoals; try eassumption.
     enough (Pa Δ {{{ IT[Id] }}}) by (eapply glu_sort_elem_typ_resp_exp_eq; mauto 3).
-    (* eapply H36; mauto 3.     *)
     eapply H36; mauto 3.
   }
 
@@ -782,9 +648,7 @@ Proof.
   }
   assert {{ Δ ⊢s σ∘Id,,N[σ] ® ρ ↦ n ∈ SbΓA }} as Hcons.
   {
-    (* eapply H43. *)
     eapply H49.
-    (* eapply cons_glu_sub_pred_helper; only 1-2: rewrite H7; mauto 3. *)
     eapply cons_glu_sub_pred_helper_sorted; only 1-2: rewrite H6; mauto 3.
     enough (SbΓ'' Δ σ ρ) by (eapply glu_ctx_env_sub_resp_sub_eq; mauto 4); eassumption.
     econstructor; mauto 2.
@@ -821,36 +685,6 @@ Proof.
   eapply glu_sort_elem_typ_unique_upto_exp_eq; revgoals; eassumption.
 Qed.
 
-(* Lemma glu_rel_exp_app {P} (pred_P : PredicativeSig P) (full_P : FullSig P) : forall {Γ M N A B s1 s2 s3 s2'} {r : Ru P s1 s2 s3}, *)
-(*     {{ ⟪ pred_P ⟫ Γ, A@s1 ⊩ B : Sort@s2 @ s2' }} -> *)
-(*     {{ ⟪ pred_P ⟫ Γ ⊩ M : Π r A B @ s3 }} -> *)
-(*     {{ ⟪ pred_P ⟫ Γ ⊩ N : A @ s1 }} -> *)
-(*     {{ ⟪ pred_P ⟫ Γ ⊩ M N : B[Id,,N] @ s2 }}. *)
-(* Proof. *)
-(*   intros * HB HM HN. *)
-(*   assert {{ ⟪ pred_P ⟫ ⊩ Γ, A@s1 }} as [SbΓA] by mauto 3. *)
-(*   match_by_head (glu_ctx_env pred_P SbΓA) invert_glu_ctx_env. *)
-(*   apply_predicate_equivalence. *)
-(*   rename TSb into SbΓ. *)
-(*   assert (exists s1', Ax P s1 s1') as [s1'] by (eapply full_P). *)
-(*   assert {{ ⟪ pred_P ⟫ Γ ⊩ A : Sort@s1 @ s1' }}. *)
-(*   { *)
-(*     eexists. *)
-(*     intuition. *)
-(*     destruct_glu_rel_typ_with_sub. *)
-(*     econstructor; mauto 4. *)
-(*     econstructor; [| split]; mauto 3. *)
-(*     eapply wf_exp_sub_typ; mauto 3. *)
-(*     do 2 eexists; mauto 2. *)
-(*   } *)
-(*   assert {{ ⟪ pred_P ⟫ ⊩ Γ }} by mauto 2. *)
-(*   assert {{ ⟪ pred_P ⟫ ⊩ Γ, A@s1 }} by mauto 3. *)
-(*   mauto 2 using glu_rel_exp_app_helper. *)
-(* Qed. *)
-
-(* #[export] *)
-(* Hint Resolve glu_rel_exp_app : mcpts. *)
-
 
 Lemma glu_rel_exp_app_helper_unsorted {P} (pred_P : PredicativeSig P) : forall {anns Γ M N A B s1 s2 s3} {r : Ru_pi P s1 s2 s3},
     {{ ⟪ pred_P ⟫ Γ with anns ⊩u A : Sort@s1 @ ^so_None }} ->
@@ -861,7 +695,6 @@ Lemma glu_rel_exp_app_helper_unsorted {P} (pred_P : PredicativeSig P) : forall {
 Proof.
   intros * HA HB HM HN.
   assert {{ ⟪ pred_P ⟫ ⊩ Γ with anns }} as [SbΓ] by mauto 3.
-  (* assert (exists s3', {{ ⟪ pred_P ⟫ Γ ⊩ Π r A B : Sort@s3 @ s3' }}) as [s3'] by mauto 4. *)
   assert {{ Γ ⊢ N : A }} by mauto 2.
   inversion_clear HN as [SbΓ' []].
   handle_functional_glu_ctx_env P.
@@ -886,8 +719,6 @@ Proof.
   handle_functional_glu_ctx_env P.
   eexists; split; [eassumption |].
   intros.
-  (* assert (SbΓ Δ σ ρ) by (eapply H7; mauto 2). *)
-  (* assert (SbΓ' Δ σ ρ) by (eapply H13; mauto 2). *)
   assert (SbΓ Δ σ ρ) by (eapply H6; mauto 2).
   assert (SbΓ' Δ σ ρ) by (eapply H12; mauto 2).
   destruct_glu_rel_exp_with_sub_unsorted.
@@ -900,8 +731,6 @@ Proof.
 
   match_by_head (@glu_sort_elem) ltac:(fun H => directed invert_glu_sort_elem H).
   simpl_glu_rel.
-
-
   assert (glu_sort_elem pred_P s1 IP IEL a).
   {
     assert ((pred_rel pred_P s1 s3 \/ s1 = s3) /\ (pred_rel pred_P s2 s3 \/ s2 = s3)) as [pr1 pr2] by (eapply ord_ru_pi; mauto 2).
@@ -919,14 +748,9 @@ Proof.
   }
 
   apply_predicate_equivalence.
-  (* unfold sort_glu_exp_pred' in *. *)
-  (* unfold glu_sort_typ_rec in *. *)
-  (* destruct_conjs. *)
   simpl_glu_rel.
   handle_functional_glu_sort_elem P.
   match_by_head (@per_sort_elem P) ltac:(fun H => directed invert_per_sort_elem H).
-  (* inversion_clear H22. *)
-  (* inversion_clear H21. *)
   match goal with
   | _: glu_sort_elem pred_P s1 ?P' ?El' a,
       _: {{ ⟦ A ⟧ ρ ↘ ^?a' }},
@@ -953,22 +777,6 @@ Proof.
   (on_all_hyp: destruct_rel_by_assumption in_rel0).
   simplify_evals.
 
-  (* pose proof H7. *)
-  (* invert_glu_ctx_env H21. *)
-  (* assert (cons_glu_sub_pred pred_P s1 Γ A TSb Δ {{{ σ,,N[σ] }}} d{{{ ρ ↦ n }}}) as Hconspred. *)
-  (* { *)
-  (*   eapply cons_glu_sub_pred_helper; mauto 3. *)
-  (*   handle_functional_glu_ctx_env P. *)
-  (*   eassumption. *)
-  (* } *)
-  (* eapply H28 in Hconspred. *)
-  (* pose proof (H8 _ _ _ Hconspred). *)
-  (* inversion H29. *)
-  (* inversion H30. *)
-  (* subst. *)
-  (* rename s into s2. *)
-
-
   match goal with
   | _: {{ ⟦ B ⟧ ρ ↦ n ↘ ^?b' }},
       _: {{ $| m & n |↘ ^?mn' }} |- _ =>
@@ -991,7 +799,6 @@ Proof.
   {
     autorewrite with mcpts; eapply glu_sort_elem_typ_unique_upto_exp_eq; revgoals; try eassumption.
     enough (Pa Δ {{{ IT[Id] }}}) by (eapply glu_sort_elem_typ_resp_exp_eq; mauto 3).
-    (* eapply H36; mauto 3.     *)
     eapply H32; mauto 3.
   }
 
@@ -1004,26 +811,15 @@ Proof.
   {
     eapply glu_ctx_env_cons_clean_inversion; mauto 3.
   }
-  (* (* rewrite H7. *) *)
-  (*   rewrite H6. *)
-  (*   eassumption. *)
-  (* } *)
   assert {{ Δ ⊢s σ∘Id,,N[σ] ® ρ ↦ n ∈ SbΓA }} as Hcons.
   {
-    (* eapply H43. *)
     eapply H51.
-    (* eapply cons_glu_sub_pred_helper; only 1-2: rewrite H7; mauto 3. *)
     eapply cons_glu_sub_pred_helper_sorted; mauto 3.
     - eapply glu_ctx_env_sub_monotone; mauto 3.
     - econstructor; mauto 3.
     - assert {{ Δ ⊢ A[σ∘Id] ≈ A[σ] : Sort@s1 }} as -> by mauto 4.
       mauto 2.
   }
-  (*   only 1-2: rewrite H6; mauto 3. *)
-  (*   enough (SbΓ'' Δ σ ρ) by (eapply glu_ctx_env_sub_resp_sub_eq; mauto 4); eassumption. *)
-  (*   assert {{ Δ ⊢ A[σ∘Id] ≈ A[σ][Id] : Sort@s1 }} by (eapply exp_eq_sub_compose_typ_sort; mauto 3). *)
-  (*   enough (Ela Δ {{{ A[σ][Id] }}} {{{ N[σ] }}} n) by (eapply glu_sort_elem_trm_resp_typ_exp_eq; mauto 3); eassumption.     *)
-  (* } *)
   pose proof (H8 _ _ _ Hcons).
   inversion H52.
   inversion H53.
@@ -1031,7 +827,6 @@ Proof.
   inversion H65; subst.
   rename s into s2.
 
-  (* (on_all_hyp: destruct_glu_rel_by_assumption SbΓA). *)
   simplify_evals.
   match_by_head (@glu_sort_elem P) ltac:(fun H => directed invert_glu_sort_elem H).
   apply_predicate_equivalence.
