theories/Core/Soundness/Realizability.v
@@ -61,22 +61,17 @@ Proof.
 
   - pose proof (app_ctx_vlookup _ _ _ _ HΔ0 eq_refl) as Hvar.
     pose proof (app_ctx_lookup Γ1 A0 Γ2 _ eq_refl).
-
-    (* gen_presup Hvar. *)
     clear_dups.
     assert {{ ⊢ Δ', A }} by mauto 3.
     assert {{ Δ', A ⊢s Wk : ^(Γ1 ++ {{{ Γ2, A0 }}}) }} by mauto 3.
     transitivity {{{ #(length Γ1)[Wk∘τ] }}}; [mauto 5 |].
     assert {{ Γ ⊢ ^ (iter (S (length Γ1)) (fun A1 : exp P => {{{ A1[Wk] }}}) A0)[Wk∘τ] ≈ ^ (iter (S (length Γ1)) (fun A1 : exp P => {{{ A1[Wk] }}}) A0)[σ] }} by mauto 5.
     eapply wf_exp_eq_conv'; mauto 2.
-    (* eapply wf_exp_eq_conv' with (A := {{{ ^ (iter (S (length Γ1)) (fun A1 : exp P => {{{ A1[Wk] }}}) A0)[Wk∘τ] }}}); mauto 4. *)
 
     etransitivity; [eapply wf_exp_eq_sub_compose_typ; mauto 3 |].
     pose proof (wf_ctx_sub_length _ _ H0).
-
     assert {{ Γ ⊢ ^ (iter (S (length Γ1)) (fun A1 : exp P => {{{ A1[Wk] }}}) A0)[Wk][τ] ≈ ^ (iter (S (length Γ1)) (fun A1 : exp P => {{{ A1[Wk] }}}) A0)[Wk∘τ] }} by mauto 5.
     eapply wf_exp_eq_conv'; mauto 2.
-    (* eapply wf_exp_eq_conv' with (A := {{{ ^ (iter (S (length Γ1)) (fun A1 : exp P => {{{ A1[Wk] }}}) A0)[Wk][τ] }}}); mauto 4. *)
 
     deepexec (@wf_ctx_sub_ctx_lookup P) ltac:(fun H => destruct H as [Γ1' [? [Γ2' [? [-> [? [-> []]]]]]]]).
     repeat rewrite List.length_app in *.
@@ -217,7 +212,6 @@ Proof.
       simplify_evals.
       assert (per_sort_elem pred_P s2 (out_rel d{{{ ⇑! a (length Δ) }}} d{{{ ⇑! a (length Δ) }}} H29) b b) by (destruct_conjs; pose proof ord_ru_pi_sub pred_P r sub_s3_s as [? []]; subst; mauto 2).
       
-      (* destruct (H2 _ ltac:(eassumption) _ ltac:(eassumption)) as [? []]. *)
       assert (IEL {{{ Δ, IT[σ] }}} {{{ IT[σ][Wk] }}} {{{ #0 }}} d{{{ ⇑! a (length Δ) }}}) by mauto 3 using var_glu_elem_bot.
       assert {{ Δ, IT[σ] ⊢ IT[σ][Wk] ≈ IT[σ∘Wk] : Sort@s1 }}.
       {
@@ -308,9 +302,6 @@ Proof.
            bulky_rewrite_in H17.
         -- assert (wf_typ_eq Δ0 {{{ IT[σ][σ0] }}} {{{ IT[σ∘σ0] }}}) by mauto.
            eapply wf_exp_eq_conv'; mauto 3.
-        (* -- assert (wf_typ Δ0 {{{ IT[σ∘σ0] }}}) by mauto. *)
-        (*    assert (wf_typ Δ0 {{{ IT[σ][σ0] }}}) by mauto 4. *)
-        (*    econstructor; mauto 3. *)
 
   - handle_functional_glu_sort_elem P.
     handle_per_sort_elem_irrel.
@@ -385,69 +376,6 @@ Proof.
         assert {{ Δ, IT[σ] ⊢ OT[σ∘Wk,,#0] ® glu_typ_top pred_P s2 b }}  as [] by mauto 3.
         assert ({{ Δ, IT[σ] ⊢ OT[σ∘Wk,,#0][Id] ≈ B' : Sort@s2 }}) by mauto 4.
         mauto 4.
-      (* * gen_presup H50; econstructor; mauto 3. *)
-        
-      
-      
-
-      
-      
-      (* specialize (H29 _ _ _ H20 H9). *)
-      (* assert (in_rel0 d{{{ ⇑! a (length Δ) }}} d{{{ ⇑! a (length Δ) }}}) by (eapply per_bot_then_per_elem; mauto 2). *)
-      (* assert (in_rel d{{{ ⇑! a (length Δ) }}} d{{{ ⇑! a (length Δ) }}}) by intuition. *)
-      (* destruct_rel_mod_eval. *)
-      (* simplify_evals. *)
-      (* assert (per_sort_elem pred_P s2 (out_rel d{{{ ⇑! a (length Δ) }}} d{{{ ⇑! a (length Δ) }}} H30) b b) by (pose proof ord_ru_pi_sub pred_P r sub_s3_s as [? []]; subst; mauto 2). *)
-
-      (* specialize (H1 _ H31 _ H22). *)
-      (* specialize (H2 _ H31 _ H22) as [? []]. *)
-      
-      (* rewrite H29 in *. *)
-      (* autorewrite with mcpts. *)
-      (* eassert (wf_exp Δ _ {{{ M[σ] }}}) by mauto 3. *)
-      (* autorewrite with mcpts in H30. *)
-      (* rewrite @wf_exp_eq_pi_eta' with (M := {{{ M[σ] }}}); [| trivial]. *)
-      (* cbn [nf_to_exp]. *)
-      (* eapply wf_exp_eq_fn_cong'; eauto; [| mauto 4]. *)
-      (* pose proof (var_per_elem (length Δ) H0). *)
-      (* destruct_rel_mod_eval. *)
-      (* simplify_evals. *)
-      (* destruct (H2 _ ltac:(eassumption) _ ltac:(eassumption)) as [? []]. *)
-      (* specialize (H12 _ _ _ _ ltac:(trivial) (var_glu_elem_bot _ _ _ _ _ _ _ H H10)). *)
-      (* assert (IEL {{{ Δ,IT[σ]@s1 }}} {{{ IT[σ∘Wk] }}} {{{ #0 }}} d{{{ ⇑! a (length Δ) }}}). *)
-      (* { *)
-      (*   eapply glu_sort_elem_trm_resp_typ_exp_eq; mauto 3. *)
-      (*   symmetry. *)
-      (*   eapply exp_eq_sub_compose_typ_sort; mauto 4. *)
-      (* } *)
-      (* specialize (H14 {{{Δ, IT[σ]@s1 }}} {{{σ ∘ Wk}}} _ _ ltac:(mauto) ltac:(eassumption) ltac:(eassumption)) as [? []]. *)
-      (* apply_equiv_left. *)
-      (* destruct_rel_mod_app. *)
-      (* simplify_evals. *)
-      (* deepexec H1 ltac:(fun H => pose proof H). *)
-      (* specialize (H33 _ _ _ _ _ ltac:(eassumption) ltac:(eassumption) ltac:(eassumption) ltac:(eassumption)) as []. *)
-      (* specialize (H41 _ {{{Id}}} _ ltac:(mauto 3) ltac:(eassumption)). *)
-      (* do 2 (rewrite wf_exp_eq_sub_id in H41; mauto 4). *)
-      (* etransitivity; [|eassumption]. *)
-      (* simpl. *)
-      (* assert (wf_exp {{{ Δ, IT[σ]@s1 }}} {{{ IT[σ∘Wk] }}} (@a_var P 0)). *)
-      (* { *)
-      (*   eapply wf_conv' with (A := {{{ IT[σ][Wk] }}}); mauto 3. *)
-      (*   symmetry; eapply wf_exp_eq_sub_compose_sort; mauto 3. *)
-      (* } *)
-      (* rewrite <- @sub_eq_q_sigma_id_extend; mauto 4. *)
-      (* assert (wf_exp {{{ Γ, IT@s1 }}} {{{ Sort@s2 }}} OT ) by mauto 3. *)
-      (* assert (wf_sub Δ Γ σ) by mauto 3. *)
-      (* assert (wf_sub {{{ Δ, IT[σ]@s1 }}} Δ {{{ Wk }}}) by mauto 3. *)
-      (* assert (wf_sub {{{ Δ, IT[σ]@s1 }}} Γ {{{ σ ∘ Wk }}}) by mauto 3. *)
-      (* assert (wf_sub {{{ Δ, IT[σ]@s1, IT[σ∘Wk]@s1 }}} {{{ Γ, IT@s1 }}} {{{ q (σ∘Wk ) }}}) by mauto 3. *)
-      (* assert (wf_exp {{{ Δ, IT[σ]@s1 }}} {{{ IT[σ∘Wk] }}} {{{ #0 }}}) by mauto 3. *)
-      (* assert (wf_sub {{{ Δ, IT[σ]@s1 }}} {{{ Δ, IT[σ]@s1, IT[σ∘Wk]@s1 }}} {{{ Id,,#0 }}}) by mauto 4. *)
-      (* assert (wf_exp_eq {{{ Δ, IT[σ]@s1 }}} {{{ Sort@s2 }}} {{{ OT[q (σ∘Wk)∘(Id,,#0)] }}} {{{ OT[q (σ∘Wk)][Id,,#0] }}}) by (symmetry; mauto 3). *)
-      (* eapply wf_exp_eq_conv' with (A := {{{ OT[q (σ∘Wk)][Id,,#0] }}}); mauto 2. *)
-      (* eapply wf_exp_eq_app_cong'; [| mauto 3]. *)
-      (* symmetry. *)
-      (* rewrite <- wf_exp_eq_pi_sub; mauto 4. *)
       
   - econstructor; eauto; intros.
     progressive_inversion.
@@ -688,4 +616,14 @@ Proof.
   - intros.
     progressive_inversion.
     exact (var_weaken_gen _ _ _ H2 nil _ _ eq_refl).
+Qed.
+
+Corollary var0_glu_elem_unsorted {P} (pred_P : PredicativeSig P) : forall {a typ_rel exp_rel Γ A},
+    {{ DG a ∈ glu_typ_elem pred_P so_None ↘ typ_rel ↘ exp_rel }} ->
+    {{ Γ ⊢ A ® typ_rel }} ->
+    {{ Γ, A ⊢ #0 : A[Wk] ® ⇑! a (length Γ) ∈ exp_rel }}.
+Proof.
+  intros.
+  eapply realize_glu_elem_bot_unsorted; mauto 4.
+  eauto using var_glu_elem_bot_unsorted.
 Qed.
