theories/Core/Soundness/SortCases.v
@@ -5,24 +5,6 @@ From McPTS.Core.Semantic Require Import Realizability.
 From McPTS.Core.Soundness Require Import LogicalRelation TermStructureCases.
 Import Domain_Notations.
 
-(* Lemma glu_rel_exp_of_typ {P} (pred_P : PredicativeSig P) (full_P : FullSig P) : forall {Γ Sb A s s'}, *)
-(*     Ax P s s' -> *)
-(*     {{ EG Γ ∈ glu_ctx_env pred_P ↘ Sb }} -> *)
-(*     (forall Δ σ ρ, *)
-(*         {{ Δ ⊢s σ ® ρ ∈ Sb }} -> *)
-(*         {{ Δ ⊢ A[σ] : Sort@s }} /\ *)
-(*           exists a, *)
-(*             {{ ⟦ A ⟧ ρ ↘ a }} /\ *)
-(*               {{ Dom a ≈ a ∈ per_sort pred_P s }} /\ *)
-(*               forall typ_rel exp_rel, {{ DG a ∈ glu_sort_elem pred_P s ↘ typ_rel ↘ exp_rel }} -> {{ Δ ⊢ A[σ] ® typ_rel }}) -> *)
-(*       {{ ⟪ pred_P ⟫ Γ ⊩ A : Sort@s @ s' }}. *)
-(* Proof. *)
-(*   intros * Hax ? Hbody. *)
-(*   eexists; split; mauto. *)
-(*   intros. *)
-(*   edestruct Hbody as [? [? [? []]]]; mauto. *)
-(* Qed. *)
-
 
 Lemma glu_rel_exp_of_typ_unsorted {P} (pred_P : PredicativeSig P) : forall {anns Γ Sb A s},
     {{ EG Γ ∈ glu_ctx_env pred_P anns ↘ Sb }} ->
@@ -47,29 +29,6 @@ Proof.
     specialize (H4 typ_rel exp_rel H5).
     eassumption.
 Qed.
-
-
-(* Lemma glu_rel_exp_typ {P} (pred_P : PredicativeSig P) (full_P : FullSig P) : forall {Γ s s' s''}, *)
-(*     Ax P s s' -> Ax P s' s'' -> *)
-(*     {{ ⟪ pred_P ⟫ ⊩ Γ }} -> *)
-(*     {{ ⟪ pred_P ⟫ Γ ⊩ Sort@s : Sort@s' @ s'' }}. *)
-(* Proof. *)
-(*   intros * Hax Hax' []. *)
-(*   eapply glu_rel_exp_of_typ; mauto 3. *)
-(*   intros. *)
-(*   assert {{ Δ ⊢s σ : Γ }} by mauto 3. *)
-(*   split; mauto 4. *)
-(*   eexists; repeat split; mauto. *)
-(*   intros. *)
-(*   match_by_head1 (@glu_sort_elem P) invert_glu_sort_elem. *)
-(*   apply_predicate_equivalence. *)
-(*   cbn. *)
-(*   mauto 4. *)
-(* Qed. *)
-
-(* #[export] *)
-(* Hint Resolve glu_rel_exp_typ : mcpts. *)
-
 
 Lemma glu_rel_exp_typ_unsorted {P} (pred_P : PredicativeSig P) : forall {anns Γ s s'},
     Ax_typ P s s' ->
