theories/Core/Syntactic/SystemAnnotated.v
@@ -1,0 +1,1 @@
+From McPTS.Core.Syntactic.SystemAnnotated Require Export Definitions Lemmas.
